# Quadratic Formula

The quadratic formula is given by:

$$
x = \frac{{-b \pm \sqrt{{b^2 - 4ac}}}}{{2a}}
$$

where:
- \( a \) is the coefficient of \( x^2 \)
- \( b \) is the coefficient of \( x \)
- \( c \) is the constant term

### Example Calculation

For the quadratic equation \( x^2 + 3x + 2 = 0 \):

1. Coefficients are \( a = 1 \), \( b = 3 \), and \( c = 2 \).
2. The solution is:

$$
x = \frac{{-3 \pm \sqrt{{3^2 - 4 \cdot 1 \cdot 2}}}}{{2 \cdot 1}} = \frac{{-3 \pm \sqrt{1}}}{2}
$$

This gives us the roots \( x = -1 \) and \( x = -2 \).

